proof/SimMemId.v
@@ -12,7 +12,8 @@ Require Import AST.
 Require Import Asmregs.
 Require Import Integers.
 
-Require Import Skeleton Mod ModSem.
+Require Import IntegersC LinkingC.
+Require Import SimDef SimSymb Skeleton Mod ModSem.
 Require Import SimMem.
 
 Set Implicit Arguments.
@@ -52,4 +53,144 @@ Qed.
 (*   - admit "This should hold; Maybe ""Genv.init_mem_match"" and ""Genv.init_mem_genv_next"" might help". *)
 (*   - admit "This should hold;". *)
 (* Qed. *)
+
+
+
+
+
+
+
+
+
+
+
+
+
+
+
+
+
+Inductive sim_skenv (skenv0 skenv1: SkEnv.t): Prop :=
+| sim_skenv_intro
+    (NEXT: skenv0.(Genv.genv_next) = skenv1.(Genv.genv_next))
+    (SYMB: all1 (skenv0.(Genv.find_symbol) =1= skenv1.(Genv.find_symbol)))
+    (DEFS: all1 (skenv0.(Genv.find_def) =1= skenv1.(Genv.find_def)))
+    (PUBS: skenv0.(Genv.genv_public) = skenv1.(Genv.genv_public))
+.
+
+Goal sim_skenv = Genv.match_genvs eq.
+Proof.
+  apply Axioms.functional_extensionality; i.
+  apply Axioms.functional_extensionality; i.
+  apply AxiomsC.prop_ext.
+  split; i; inv H; econs; eauto.
+  - ii. unfold Genv.find_def in *. erewrite DEFS.
+    destruct ((Genv.genv_defs x0) ! b) eqn:T; econs; eauto.
+  - unfold Genv.find_def in *. i. specialize (mge_defs x1). inv mge_defs; ss.
+  - admit "".
+Qed.
+
+Inductive sim_sk (u: unit) (sk_src sk_tgt: Sk.t): Prop :=
+| sim_sk_intro
+    (SIM: match_program (fun _ => sim_fun) eq sk_src sk_tgt)
+.
+
+Global Program Instance SimSymbId: SimSymb.class SimMemId := {
+  t := unit;
+  le := top4;
+  sim_sk := sim_sk;
+  sim_skenv (_: SimMem.t) (_: unit) := sim_skenv;
+}
+.
+Next Obligation.
+  inv SIMSK. inv SIMSK0.
+  SearchAbout TransfLink.
+  admit "this should hold".
+Qed.
+Next Obligation.
+  u in *. inv SIMSK.
+  Print Genv.init_mem_transf.
+  Print Genv.init_mem_transf_partial.
+  About Genv.init_mem_match.
+  exploit (Genv.init_mem_match SIM); eauto. i. clarify.
+  esplits; eauto.
+  - econs; eauto.
+    + erewrite ! Genv.init_mem_genv_next; eauto.
+    + i. symmetry. apply (Genv.find_symbol_match SIM).
+    + ii. hexploit (Genv.find_def_match_2 SIM x0); eauto. intro REL.
+      inv REL; ss. inv H2; ss.
+      * admit "remove sig then this will hold // or just now this will hold if we don't drop sig on opt".
+      * inv H3; ss.
+    + inv SIM; des; ss. rewrite ! Genv.globalenv_public. ss.
+  - instantiate (1:= mk _ _). ss.
+  - ss.
+  - ss.
+Unshelve.
+Qed.
+Next Obligation.
+  inv LESRC.
+  inv LETGT.
+  inv SIMSKENV.
+  inv SIMSK. unfold match_program in *.
+  assert(DEFSEQ: sk_src.(defs) = sk_tgt.(defs)).
+  { apply Axioms.functional_extensionality. intro id.
+    hexploit (@match_program_defmap _ _ _ _ _ _ _ _ _ _ _ SIM).
+    instantiate (1:= id).
+    i.
+    inv H; ss.
+    - unfold defs.
+      admit "this is weak. add list_norept or prove my own theorem with induction.".
+    - admit "this will hold".
+  }
+  econs; eauto.
+  - eq_closure_tac.
+  - intro id.
+    destruct (Classical_Prop.classic (sk_src.(defs) id)); cycle 1.
+    + exploit SYMBDROP; eauto. i; des.
+      exploit SYMBDROP0; eauto. { rewrite <- DEFSEQ. eauto. } i; des.
+      rewrite H0. rewrite H1. ss.
+    + exploit SYMBKEEP; eauto. i; des.
+      exploit SYMBKEEP0; eauto. { rewrite <- DEFSEQ. eauto. } i; des.
+      rewrite H0. rewrite H1. ss.
+  - intro blk.
+    destruct (Genv.invert_symbol skenv_link_src blk) eqn:T0; cycle 1.
+    + rewrite DEFORPHAN; ss.
+      destruct (Genv.invert_symbol skenv_link_tgt blk) eqn:T1; cycle 1.
+      * rewrite DEFORPHAN0; ss.
+      * repeat all_once_fast ltac:(fun H => try apply Genv.invert_find_symbol in H; des).
+        rewrite <- SYMB in *.
+        repeat all_once_fast ltac:(fun H => try apply Genv.find_invert_symbol in H; des).
+        clarify.
+    + destruct (Genv.invert_symbol skenv_link_tgt blk) eqn:T1; cycle 1.
+      * repeat all_once_fast ltac:(fun H => try apply Genv.invert_find_symbol in H; des).
+        rewrite SYMB in *.
+        repeat all_once_fast ltac:(fun H => try apply Genv.find_invert_symbol in H; des).
+        clarify.
+      * repeat all_once_fast ltac:(fun H => try apply Genv.invert_find_symbol in H; des).
+        assert(i = i0).
+        { eapply Genv.genv_vars_inj; eauto. unfold Genv.find_symbol in *. rewrite SYMB. ss. }
+        clarify.
+        repeat all_once_fast ltac:(fun H => try apply Genv.find_invert_symbol in H; des).
+        destruct (classic (defs sk_src i0)).
+        { erewrite DEFKEEP; eauto. erewrite DEFKEEP0; eauto. rewrite <- DEFSEQ; ss. }
+        { erewrite DEFDROP; eauto. erewrite DEFDROP0; eauto. rewrite <- DEFSEQ; ss. }
+  - eq_closure_tac. ss. (* TODO: debug this *)
+    rewrite PUBLIC. rewrite PUBS. rewrite PUBLIC0. ss.
+Qed.
+Next Obligation.
+  inv SIMSKENV.
+  econs; eauto.
+  - ii. ss.
+    assert(fptr_src = fptr_tgt).
+    { ss. }
+    clarify. unfold Genv.find_funct, Genv.find_funct_ptr in *. des_ifs_safe.
+    erewrite <- DEFS; eauto. des_ifs. esplits; eauto.
+    admit "just use eq".
+  - ii.
+    assert(fptr_src = fptr_tgt).
+    { ss. }
+    clarify. unfold Genv.find_funct, Genv.find_funct_ptr in *. des_ifs_safe.
+    erewrite DEFS; eauto. des_ifs. esplits; eauto.
+    admit "just use eq".
+Qed.
 
