proof/SimMemInj.v
@@ -6,6 +6,8 @@ Require Import Events.
 Require Import Globalenvs.
 Require Import AST.
 
+Require Import IntegersC LinkingC.
+Require Import SimDef SimSymb Skeleton Mod ModSem.
 Require Import SimMem.
 
 Set Implicit Arguments.
@@ -125,7 +127,7 @@ Section MEMINJ.
 Local Existing Instance Val.mi_normal.
 (* Variable gbound_src gbound_tgt: block. *)
 
-Record t' := mkrelation {
+Record t' := mk {
   inj: meminj; (* public memory injection *)
   src_private: forall (b: block) (ofs: Z), Prop; (* source private memory *)
   tgt_private: forall (b: block) (ofs: Z), Prop; (* target private memory *)
@@ -173,14 +175,14 @@ Inductive le' (mrel0 mrel1: t'): Prop :=
 .
 
 Definition lift' (mrel0: t'): t' :=
-  (mkrelation mrel0.(inj) (fun _ _ => False) (fun _ _ => False)
+  (mk mrel0.(inj) (fun _ _ => False) (fun _ _ => False)
                           (mrel0.(src_private) \2/ mrel0.(src_external))
                           (mrel0.(tgt_private) \2/ mrel0.(tgt_external))
                           mrel0.(src_mem) mrel0.(tgt_mem) mrel0.(src_mem) mrel0.(tgt_mem))
 .
 
 Definition unlift' (mrel0 mrel1: t'): t' :=
-  (mkrelation mrel1.(inj)
+  (mk mrel1.(inj)
                       (mrel0.(src_private)) (mrel0.(tgt_private))
                       (mrel0.(src_external)) (mrel0.(tgt_external))
                       mrel1.(src_mem) mrel1.(tgt_mem) mrel0.(src_mem_parent) mrel0.(tgt_mem_parent))
@@ -306,3 +308,185 @@ Next Obligation.
 Qed.
 
 End MEMINJ.
+
+
+
+
+
+
+
+
+
+
+
+
+
+Inductive sim_skenv (skenv0 skenv1: SkEnv.t): Prop :=
+| sim_skenv_intro
+    (NEXT: skenv0.(Genv.genv_next) = skenv1.(Genv.genv_next))
+    (SYMB: all1 (skenv0.(Genv.find_symbol) =1= skenv1.(Genv.find_symbol)))
+    (DEFS: all1 (skenv0.(Genv.find_def) =1= skenv1.(Genv.find_def)))
+    (PUBS: skenv0.(Genv.genv_public) = skenv1.(Genv.genv_public))
+.
+
+Inductive skenv_inject (skenv: SkEnv.t) (j: meminj): Prop :=
+| sken_inject_intro
+    (DOMAIN: forall b, Plt b skenv.(Genv.genv_next) -> j b = Some(b, 0))
+    (IMAGE: forall b1 b2 delta, j b1 = Some(b2, delta) -> Plt b2 skenv.(Genv.genv_next) -> b1 = b2)
+.
+
+Inductive sim_skenv_inj (sm: SimMem.t) (__noname__: unit) (skenv_src skenv_tgt: SkEnv.t): Prop :=
+| sim_skenv_inj_intro
+    (INJECT: skenv_inject skenv_src sm.(inj))
+    (BOUNDSRC: Ple skenv_src.(Genv.genv_next) sm.(src_mem_parent).(Mem.nextblock))
+    (BOUNDTGT: Ple skenv_src.(Genv.genv_next) sm.(tgt_mem_parent).(Mem.nextblock))
+    (SIMSKENV: sim_skenv skenv_src skenv_tgt)
+.
+
+Inductive sim_sk (u: unit) (sk_src sk_tgt: Sk.t): Prop :=
+| sim_sk_intro
+    (SIM: match_program (fun _ => sim_fun) eq sk_src sk_tgt)
+.
+
+Global Program Instance SimSymbId: SimSymb.class SimMemInj := {
+  t := unit;
+  le := top4;
+  sim_sk := sim_sk;
+  sim_skenv := sim_skenv_inj;
+}
+.
+Next Obligation.
+  inv SIMSK. inv SIMSK0.
+  SearchAbout TransfLink.
+  admit "this should hold".
+Qed.
+Next Obligation.
+  u in *. inv SIMSK.
+  Print Genv.init_mem_transf.
+  Print Genv.init_mem_transf_partial.
+  About Genv.init_mem_match.
+  exploit (Genv.init_mem_match SIM); eauto. i. clarify.
+  esplits; eauto.
+  - instantiate (1:= mk (Mem.flat_inj m_src.(Mem.nextblock))
+                                  bot2 bot2 bot2 bot2 m_src m_src m_src m_src).
+    econs; ss; eauto.
+    + econs; eauto; ii; ss.
+      * unfold Mem.flat_inj in *. erewrite ! Genv.init_mem_genv_next in *; eauto. des_ifs.
+      * unfold Mem.flat_inj in *. erewrite ! Genv.init_mem_genv_next in *; eauto. des_ifs.
+    + ss. erewrite ! Genv.init_mem_genv_next; eauto. reflexivity.
+    + ss. erewrite ! Genv.init_mem_genv_next; eauto. reflexivity.
+    + econs; eauto.
+      * erewrite ! Genv.init_mem_genv_next; eauto.
+      * i. symmetry. apply (Genv.find_symbol_match SIM).
+      * ii. hexploit (Genv.find_def_match_2 SIM x0); eauto. intro REL.
+        inv REL; ss. inv H2; ss.
+        { admit "remove sig then this will hold // or just now this will hold if we don't drop sig on opt". }
+        inv H3; ss.
+      * inv SIM; des; ss. rewrite ! Genv.globalenv_public. ss.
+  - ss.
+  - ss.
+  - econs; ss; try xomega; ii; des; ss; eauto.
+    eapply Genv.initmem_inject; eauto.
+Unshelve.
+Qed.
+Next Obligation.
+  assert(BOUNDSRC: Ple (Genv.genv_next skenv_src) (Mem.nextblock (src_mem_parent sm1))).
+  { inv MLE. rewrite <- SRCPARENTEQ. eapply SIMSKENV. }
+  assert(BOUNDTGT: Ple (Genv.genv_next skenv_src) (Mem.nextblock (tgt_mem_parent sm1))).
+  { inv MLE. rewrite <- TGTPARENTEQ. eapply SIMSKENV. }
+  inv SIMSKENV. inv INJECT.
+  econs; eauto.
+  econs; eauto.
+  - ii. exploit DOMAIN; eauto. i. eapply MLE; eauto.
+  - ii. inv MLE.
+    eapply IMAGE; eauto.
+    erewrite frozen_preserves_tgt; eauto.
+    eapply Plt_Ple_trans; eauto.
+Qed.
+Next Obligation.
+  inv MWF. inv SIMSKENV.
+  econs; eauto.
+  - etransitivity; try apply SRCPBOUND. ss.
+  - etransitivity; try apply TGTPBOUND. ss.
+Qed.
+Next Obligation.
+  inv LESRC.
+  inv LETGT.
+  inv SIMSKENV. inv SIMSKENV0.
+  inv SIMSK. unfold match_program in *.
+  assert(DEFSEQ: sk_src.(defs) = sk_tgt.(defs)).
+  { apply Axioms.functional_extensionality. intro id.
+    hexploit (@match_program_defmap _ _ _ _ _ _ _ _ _ _ _ SIM).
+    instantiate (1:= id).
+    i.
+    inv H; ss.
+    - unfold defs.
+      admit "this is weak. add list_norept or prove my own theorem with induction.".
+    - admit "this will hold".
+  }
+  econs; eauto.
+  { inv INJECT.
+    econs; ii; eauto.
+    - eapply DOMAIN; eauto. rewrite NEXT. ss.
+    - eapply IMAGE; eauto. rewrite NEXT. ss.
+  }
+  { rewrite <- NEXT. ss. }
+  { rewrite <- NEXT. ss. }
+  econs; eauto.
+  - eq_closure_tac.
+  - intro id.
+    destruct (Classical_Prop.classic (sk_src.(defs) id)); cycle 1.
+    + exploit SYMBDROP; eauto. i; des.
+      exploit SYMBDROP0; eauto. { rewrite <- DEFSEQ. eauto. } i; des.
+      rewrite H0. rewrite H1. ss.
+    + exploit SYMBKEEP; eauto. i; des.
+      exploit SYMBKEEP0; eauto. { rewrite <- DEFSEQ. eauto. } i; des.
+      rewrite H0. rewrite H1. ss.
+  - intro blk.
+    destruct (Genv.invert_symbol skenv_link_src blk) eqn:T0; cycle 1.
+    + rewrite DEFORPHAN; ss.
+      destruct (Genv.invert_symbol skenv_link_tgt blk) eqn:T1; cycle 1.
+      * rewrite DEFORPHAN0; ss.
+      * repeat all_once_fast ltac:(fun H => try apply Genv.invert_find_symbol in H; des).
+        rewrite <- SYMB in *.
+        repeat all_once_fast ltac:(fun H => try apply Genv.find_invert_symbol in H; des).
+        clarify.
+    + destruct (Genv.invert_symbol skenv_link_tgt blk) eqn:T1; cycle 1.
+      * repeat all_once_fast ltac:(fun H => try apply Genv.invert_find_symbol in H; des).
+        rewrite SYMB in *.
+        repeat all_once_fast ltac:(fun H => try apply Genv.find_invert_symbol in H; des).
+        clarify.
+      * repeat all_once_fast ltac:(fun H => try apply Genv.invert_find_symbol in H; des).
+        assert(i = i0).
+        { eapply Genv.genv_vars_inj; eauto. unfold Genv.find_symbol in *. rewrite SYMB. ss. }
+        clarify.
+        repeat all_once_fast ltac:(fun H => try apply Genv.find_invert_symbol in H; des).
+        destruct (classic (defs sk_src i0)).
+        { erewrite DEFKEEP; eauto. erewrite DEFKEEP0; eauto. rewrite <- DEFSEQ; ss. }
+        { erewrite DEFDROP; eauto. erewrite DEFDROP0; eauto. rewrite <- DEFSEQ; ss. }
+  - rewrite PUBLIC. rewrite PUBLIC0. ss.
+Qed.
+Next Obligation.
+  inv SIMSKENV. inv SIMSKENV0. inv INJECT.
+  econs; eauto.
+  - ii. ss.
+    assert(fptr_src = fptr_tgt).
+    { inv SIMFPTR; ss. des_ifs. rewrite Ptrofs.add_zero_l.
+      unfold Genv.find_funct, Genv.find_funct_ptr in *. des_ifs_safe.
+      exploit DOMAIN; eauto. { eapply Genv.genv_defs_range; eauto. } i; clarify. }
+    clarify. unfold Genv.find_funct, Genv.find_funct_ptr in *. des_ifs_safe.
+    erewrite <- DEFS; eauto. des_ifs. esplits; eauto.
+    admit "just use eq".
+  - ii.
+    assert(fptr_src = fptr_tgt).
+    { inv SIMFPTR; ss. des_ifs.
+      unfold Genv.find_funct, Genv.find_funct_ptr in *. des_ifs_safe.
+      exploit IMAGE; eauto. { rewrite NEXT. eapply Genv.genv_defs_range; eauto. } i; clarify.
+      exploit DOMAIN; eauto. { rewrite <- DEFS in *. eapply Genv.genv_defs_range; eauto. } i; clarify.
+      rewrite e. rewrite Ptrofs.add_zero in *. clarify.
+    }
+    clarify. unfold Genv.find_funct, Genv.find_funct_ptr in *. des_ifs_safe.
+    erewrite DEFS; eauto. des_ifs. esplits; eauto.
+    admit "just use eq".
+Qed.
+
